{
 "cells": [
  {
   "cell_type": "markdown",
   "metadata": {},
   "source": [
    "<span style=\"font-size: 14pt\">EREVAN, May-June 2017</span>\n",
    "\n",
    "<span style=\"font-size: 16pt\"> Seminar #2: Exponential smoothing models\n",
    "\n",
    "<span style=\"color:blue; font-size: 12pt\">Alexey Romanenko </span>,\n",
    "<span style=\"color:blue; font-size: 12pt; font-family: 'Verdana'\">alexromsput@gmail.com</span>\n",
    "\n",
    "\n",
    "<h1 align=\"center\"> Home Work 1 </h1>\n",
    "\n",
    "## Answer questions\n",
    "\n",
    "1) ** How do adaptive properties of SES change when smoothing parametr $\\alpha$ converges to 1?**\n",
    "\n",
    "Since $\\hat{y}_{t+1}=\\alpha y_t+(1-\\alpha)\\hat{y}_t$, thus if $\\alpha$ converges to 1, then $\\hat{y}_{t+1}\\approx y_t$. So the prediction graph just repeat original with some shift.\n",
    "\n",
    "2) ** What will be the optimal value of smoothing parameter of trend $\\beta$ in Hold model for 1) time series with slowly  changing trend; 2) stochastic changing trend (look <a href=\"http://stochastictrend.blogspot.am/\">here </a>)? **\n",
    "\n",
    "The Holt model is the following\n",
    "$$\n",
    "\\hat{y}_{t+d}=l_t+b_td,\n",
    "$$\n",
    "$$\n",
    "l_t=\\alpha y_t+(1-\\alpha)(l_{t-1}+b_{t-1})\n",
    "$$\n",
    "$$\n",
    "b_t=\\beta(l_t-l_{t-1})+(1-\\beta)b_{t-1}\n",
    "$$\n",
    "If time series has slowly changing trend, then we should take $b_t\\approx b_{t-1}$, which means that $\\beta$ should be near to $0$.\n",
    "\n",
    "If time series has stochastic changing trend, it menas that trend changes significantly during the time. Therefore in this case the optimal value of beta will be near to $1$.\n",
    "\n",
    "3) **Proof the equivalency of correction error form and smoothing form for unobserved component of TS in  Thei-Wage model (period of seasonality equals $p$):**\n",
    "\n",
    "  $$1) l_t = \\alpha (y_t - s_{t-p}) + (1-\\alpha) (l_{t-1} + b_{t-1} )=l_{t-1} + b_{t-1} + \\alpha e_t;$$\n",
    "  $$2) b_t = \\beta (l_{t} - l_{t-1} ) + (1-\\beta) b_{t-1} = b_{t-1} + \\alpha\\beta e_t;$$\n",
    "  $$3) s_t = \\gamma (y_t-l_t) + (1-\\gamma) s_{t-p} = s_{t-p} + \\gamma(1-\\alpha)e_t.$$\n",
    "\n",
    "Proof:\n",
    "\n",
    "Since $e_t=y_t-\\hat{y}_t=y_t - s_{t-p}-l_{t-1} - b_{t-1}$, thus\n",
    "$$\n",
    "1)  l_t = \\alpha (y_t - s_{t-p}) + (1-\\alpha) (l_{t-1} + b_{t-1} )=l_{t-1} + b_{t-1}+\\alpha (y_t - s_{t-p})-\\alpha (l_{t-1} + b_{t-1} )=l_{t-1} + b_{t-1}+\\alpha (y_t - s_{t-p}-l_{t-1} - b_{t-1})=l_{t-1} + b_{t-1} + \\alpha e_t.\n",
    "$$\n",
    "\n",
    "From the previous point follows that\n",
    "$$\n",
    "2) b_t = \\beta (l_{t} - l_{t-1} ) + (1-\\beta) b_{t-1} = \\beta (l_{t} - l_{t-1} ) + b_{t-1}-\\beta b_{t-1}=b_{t-1}+\\beta(l_{t} - l_{t-1}-b_{t-1})=b_{t-1} + \\alpha\\beta e_t.\n",
    "$$\n",
    "From the first point follows that\n",
    "$$\n",
    "3) s_t=\\gamma (y_t-l_t) + (1-\\gamma) s_{t-p}=\\gamma (y_t-l_t)+s_{t-p}-\\gamma s_{t-p}=s_{t-p}+\\gamma(y_t-l_t-s_{t-p})=s_{t-p}+\\gamma(y_t-s_{t-p}-l_{t-1}-b_{t-1}-\\alpha e_t)=s_{t-p}+\\gamma(e_t-\\alpha e_t)=s_{t-p} + \\gamma(1-\\alpha)e_t.\n",
    "$$\n",
    "4) **Find the correction error form for unobserved component of TS in ES with additive damped trend:**\n",
    "\n",
    "$$\\hat{y}_{t+d|t} = l_t + \\left(\\phi + \\phi^2 + \\dots + \\phi^{d}\\right) b_t.$$\n",
    "\n",
    "**Unobserved components are (in smoothing form): **\n",
    "\n",
    "$$ l_{t}       = \\alpha y_t + \\left(1-\\alpha\\right) \\left(l_{t-1} +\\phi b_{t-1}\\right),$$\n",
    "$$ b_t         = \\beta \\left(l_t - l_{t-1}\\right) + \\left(1-\\beta\\right)\\phi b_{t-1}.$$\n",
    "\n",
    "In this model we have $\\hat{y}_{t|t-1}=l_{t-1}+\\phi b_{t-1}$, thus\n",
    "$$\n",
    "e_t=y_{t}-\\hat{y}_{t|t-1}=y_{t}-l_{t-1}-\\phi b_{t-1}.\n",
    "$$\n",
    "It follows that\n",
    "$$\n",
    "l_t=\\alpha y_t + \\left(1-\\alpha\\right) \\left(l_{t-1} +\\phi b_{t-1}\\right)=\\alpha y_t+l_{t-1} +\\phi b_{t-1}-\\alpha \\left(l_{t-1} +\\phi b_{t-1}\\right)=l_{t-1} +\\phi b_{t-1}+\\alpha\\left(y_{t}-l_{t-1}-\\phi b_{t-1}\\right)=l_{t-1} +\\phi b_{t-1}+\\alpha e_t.\n",
    "$$\n",
    "From this we obtain $l_t-l_{t-1}=\\phi b_{t-1}+\\alpha e_t$, therefore\n",
    "$$\n",
    "b_t=\\beta \\left(l_t - l_{t-1}\\right) + \\left(1-\\beta\\right)\\phi b_{t-1}=\\beta \\left(\\phi b_{t-1}+\\alpha e_t\\right) + \\left(1-\\beta\\right)\\phi b_{t-1}=\\phi b_{t-1}+\\alpha\\beta e_t.\n",
    "$$"
   ]
  },
  {
   "cell_type": "code",
   "execution_count": null,
   "metadata": {
    "collapsed": true
   },
   "outputs": [],
   "source": []
  }
 ],
 "metadata": {
  "anaconda-cloud": {},
  "kernelspec": {
   "display_name": "Python 3",
   "language": "python",
   "name": "python3"
  },
  "language_info": {
   "codemirror_mode": {
    "name": "ipython",
    "version": 3
   },
   "file_extension": ".py",
   "mimetype": "text/x-python",
   "name": "python",
   "nbconvert_exporter": "python",
   "pygments_lexer": "ipython3",
   "version": "3.6.1"
  }
 },
 "nbformat": 4,
 "nbformat_minor": 1
}
